workig on test spec

rocq-brick-libcpp/proof/semaphore/spec.v
@@ -1,24 +1,26 @@
 Require Import bluerock.auto.cpp.proof.
 Require Import bluerock.brick.libcpp.semaphore.test_cpp. (* TODO: should be changed to [inc_hpp] *)
 
+Import auto_frac auto_pick_frac.
+
 Section with_cpp.
 
   Context `{Σ : cpp_logic}.
   Context  `{MOD : test_cpp.module ⊧ σ}. (* σ is the whole program *)
 
   Parameter semaphoreR : cQp.t -> gname -> Rep.
-  #[only(cfractional,timeless)] derive semaphoreR.
+  (* #[only(cfractional,timeless)] derive semaphoreR. *)
   Parameter semaphore_Val : gname -> nat -> mpred.
 
   (*Parameter mutex_token : cQp.t -> mpred.*)
 
-  (*
+  
 #[global] Declare Instance semaphoreR_cfrac : CFractional1 semaphoreR.
 #[global] Declare Instance semaphoreR_ascfrac : AsCFractional1 semaphoreR.
 #[global] Declare Instance semaphoreR_cfracvalid : CFracValid1 semaphoreR.
-#[global] Declare Instance semaphoreR_timeless : Timeless2 semaphoreR.*)
-
-  (* we might now have semaphore implemented with atomics *)
+#[global] Declare Instance semaphoreR_timeless : Timeless2 semaphoreR.
+#[global] Declare Instance semaphore_Val_affine : Affine2 semaphore_Val.
+(* we might now have semaphore implemented with atomics *)
 
   (* write this as a logically atomic triple *)
   cpp.spec "std::__1::counting_semaphore<1l>::counting_semaphore(long)" as ctor_spec with
@@ -34,43 +36,54 @@ Section with_cpp.
                   << Exists n', [|n = S n'|] ** semaphore_Val g n', COMM Q  >>
        \post Q).
 
-  (* up to here*)
-(*
-  cpp.spec "std::__1::mutex::try_acquire()" as try_lock_spec with
+  cpp.spec "std::__1::counting_semaphore<1l>::try_acquire()" as try_lock_spec with
       (\this this
-         \prepost{q R} this |-> semaphoreR q R (* part of both pre and post *)
-         \pre mutex_token q
-         \post{b}[Vbool b] if b then R else mutex_token q).
+         \prepost{q g} this |-> semaphoreR q g (* part of both pre and post *)
+         \pre{Q} AU <{ ∃∃ n, semaphore_Val g n }> @ top, empty
+                  <{ semaphore_Val g (if bool_decide (n = 0) then n else n-1), COMM Q $ bool_decide (n = 0) }>
+        \post{b}[Vbool b] (Q b)).
 
-  cpp.spec "std::__1::mutex::release()" as unlock_spec with
+  cpp.spec "std::__1::counting_semaphore<1l>::release(long)" as release_spec with
       (\this this
-         \prepost{q R} this |-> semaphoreR q R (* part of both pre and post *)
-         \pre ▷R
-         \post mutex_token q).
+        \arg{update} "update" (Vnat update)
+        \prepost{q g} this |-> semaphoreR q g
+        \pre{Q} AC << ∀ n, semaphore_Val g n ∗ [| n+update <= 1 |] >> @ top, empty
+                   << semaphore_Val g (n+update), COMM Q  >>
+       \post Q).
 
-  cpp.spec "std::__1::mutex::~mutex()" as dtor_spec with
+  cpp.spec "std::__1::counting_semaphore<1l>::~counting_semaphore()" as dtor_spec with
       (\this this
-         \with R
-               \pre this |-> semaphoreR 1$m R ** mutex_token 1$m
-               \post R).
+        \pre{g} this |-> semaphoreR 1$m g 
+        \post emp).
 
   cpp.spec "test()" as test_spec with
       (\post emp).
 
-  Declare Instance semaphoreR_typed : Typed2 "std::__1::mutex" semaphoreR.
+  Declare Instance semaphoreR_typed : Typed2 "std::__1::counting_semaphore<1l>" semaphoreR.
+
+  (* LHS learns RHS *)
+  #[global] Declare Instance inst v n : Refine1 true true (Vint v = Vnat n) ([n = Z.to_nat v]).
+  #[global] Declare Instance semaphoreR_learnable : LearnEqF1 semaphoreR.
+  
+  #[program]
+  Definition ac_C t (x:nat) :=
+    \cancelx
+    \consuming semaphore_Val t x
+    \bound_existential Q
+    \proving AC << ∀ n : nat, semaphore_Val t n >> @ ⊤, ∅
+         << ∃ n' : nat, [| n = S n' |] ∗
+          semaphore_Val t n',
+        COMM Q >>
+    \instantiate Q:=emp
+    \through ([| 0 < x |] ∗ semaphore_Val t (x - 1) -∗ emp)
+    \end.
+  Next Obligation. Admitted.
+  Hint Resolve ac_C : br_opacity.
 
   Theorem test_ok : verify[module] test_spec.
   Proof. verify_spec; go.
-         iExists emp. go. (* doesn't automatically split mutex_token *)
-         (* we could prove this without the splittable instance by manually
-       instantiating the fraction at each call to lock/unlock *)
-         iFrame.
-         go.
-         iFrame.
-         go.
-         iFrame.
-         go.
-  Qed.
-*)
+    Fail progress go using ac_C.
+  Admitted.
+
 
 End with_cpp.
